theories/algebra/pagetable.v
@@ -5,114 +5,113 @@ Section pagetable_rules.
 
   Context `{vmG :gen_VMG Σ}.
 
-(*
   (* rules for pagetables  *)
-  Lemma owned_split_set i q1 q2 (s1 s2 : gset PID):
-   s1 ## s2 -> O@i:={(q1+q2)%Qp}[(s1 ∪ s2)] -∗ O@i:={q1}[s1] ∗ O@i:={q2}[s2].
+  Lemma owned_ne p1 p2 (v1 v2 : VMID):
+   O@p1:=v1 ∗ O@p2:=v2 -∗ ⌜p1 ≠ p2⌝ .
   Proof using.
-  iIntros (Hdisj) "HO".
-  rewrite owned_mapsto_eq.
-  iApply own_op.
-  rewrite -auth_frag_op singleton_op.
-  rewrite -pair_op.
-  rewrite (gset_disj_union _ _ Hdisj).
-  naive_solver.
-  Qed.
-
-  Lemma owned_split_singleton i q1 q2 (s : gset PID) p:
-   p ∉ s -> O@i:={(q1+q2)%Qp}[(s ∪ {[p]})] -∗ O@i:={q1}[s] ∗ O@i:={q2}p.
-  Proof using.
-    iIntros (Hnotin) "HO".
-    assert (Hdisj: s ## {[p]}). { set_solver. }
-    iDestruct (owned_split_set i q1 q2 _ _ Hdisj with "HO")  as "HO'".
+    iIntros "[HO1 HO2]".
+    rewrite owned_mb_mapsto_eq /owned_mb_mapsto_def.
+    destruct (decide (p1 = p2)).
+    { subst p2.
+      iDestruct (ghost_map_elem_valid_2 with "HO1 HO2") as "[%Hvalid _]".
+      apply dfrac_valid_own_l in Hvalid.
+      inversion Hvalid.
+    }
     done.
   Qed.
-*)
- (* (* TODO *) *)
- (* Lemma access_split_set_union i q1 q2 (s1 s2 : gset PID): *)
- (*  s1 ## s2 -> *)
- (*  A@i:={(q1+q2)%Qp}[s1 ∪ s2] -∗ A@i:={q1}[s1] ∗ A@i:={q2}[s2]. *)
- (* Proof using. *)
- (*   iIntros (Hdisj) "HO". *)
- (*   rewrite access_mapsto_eq /access_mapsto_def. *)
- (*   iApply own_op. *)
- (*   rewrite -auth_frag_op singleton_op. *)
- (*   rewrite -pair_op. *)
- (*   rewrite (gset_disj_union _ _ Hdisj). *)
- (*   naive_solver. *)
- (* Qed. *)
- (* Lemma access_split_set_diff i q1 q2 (s1 s2 : gset_disj PID): *)
- (*  A@i:={(q1+q2)%Qp}[s1] -∗ A@i:={q1}[s1] ∗ A@i:={q2}[s1 ∖ s2]. *)
- (* Proof using. *)
- (*   iIntros (Hdisj) "HO". *)
- (*   rewrite access_mapsto_eq. *)
- (*   iApply own_op. *)
- (*   rewrite -auth_frag_op singleton_op. *)
- (*   rewrite -pair_op. *)
- (*   rewrite (gset_disj_union _ _ Hdisj). *)
- (*   naive_solver. *)
- (* Qed. *)
 
- (* Lemma access_split_singleton i q1 q2 (s : gset PID) p: *)
- (*  p ∉ s -> A@i:={(q1+q2)%Qp}[(s ∪ {[p]})] -∗ A@i:={q1}[s] ∗ A@i:={q2}p. *)
- (* Proof using. *)
- (*   iIntros (Hnotin) "HO". *)
- (*   assert (Hdisj: s ## {[p]}). { set_solver. } *)
- (*   iApply (access_split_set i q1 q2 _ _ Hdisj with "HO"). *)
- (* Qed. *)
-
-
-  Lemma gen_pagetable_SepM_split1 {Perm: Type} {σ γ} i (proj: page_table -> gmap PID Perm)
-        (checkb: Perm -> bool):
-   ([∗ map] k↦v ∈ (get_pagetable_gmap σ proj checkb ), ghost_map_elem γ k (dfrac.DfracOwn 1) v)%I -∗
-   ghost_map_elem γ i (dfrac.DfracOwn 1) (get_pagetable_gset σ i proj checkb) ∗
-   [∗ map] k↦v ∈ (delete i (get_pagetable_gmap σ proj checkb)), ghost_map_elem γ k (dfrac.DfracOwn 1) v.
-  Proof.
-    iIntros "Hall".
-    iApply ((big_sepM_delete _ (get_pagetable_gmap σ proj checkb) i
-                             (get_pagetable_gset σ i proj checkb)) with "Hall").
-    rewrite /get_pagetable_gmap.
-    apply elem_of_list_to_map_1.
-    {  rewrite -list_fmap_compose /compose /=. rewrite list_fmap_id. apply NoDup_list_of_vmids. }
-    rewrite elem_of_list_In.
-    rewrite in_map_iff.
-    exists i.
-    split.
-    rewrite /get_pagetable_gset //.
-    apply in_list_of_vmids.
+  Lemma access_split_set_union {p} q1 q2 (s1 s2 : gset VMID):
+   s1 ## s2 ->
+   A@p:={(q1+q2)%Qp} [s1 ∪ s2] -∗ A@p:={q1} [s1] ∗ A@p:={q2} [s2].
+  Proof using.
+    iIntros (Hdisj) "HO".
+    rewrite access_mapsto_eq /access_mapsto_def.
+    iApply own_op.
+    rewrite -auth_frag_op singleton_op.
+    rewrite -pair_op.
+    rewrite (gset_disj_union _ _ Hdisj).
+    naive_solver.
   Qed.
 
-  Lemma gen_pagetable_SepM_split2 {Perm: Type} {σ γ} i j (proj: page_table -> gmap PID Perm)
-        (checkb: Perm -> bool):
-   i ≠ j ->
-   ([∗ map] k↦v ∈ (get_pagetable_gmap σ proj checkb ), ghost_map_elem γ k (dfrac.DfracOwn 1) v)%I -∗
-   ghost_map_elem γ i (dfrac.DfracOwn 1) (get_pagetable_gset σ i proj checkb) ∗
-   ghost_map_elem γ j (dfrac.DfracOwn 1) (get_pagetable_gset σ j proj checkb) ∗
-   [∗ map] k↦v ∈ (delete j (delete i (get_pagetable_gmap σ proj checkb))),
-                  ghost_map_elem γ k (dfrac.DfracOwn 1) v.
-  Proof.
-    iIntros (Hne) "Hall".
-    iDestruct ((gen_pagetable_SepM_split1 i) with "Hall") as "[Hi Hrest]".
-    iFrame.
-    iApply ((big_sepM_delete _ _ j (get_pagetable_gset σ j proj checkb)) with "Hrest").
-    rewrite /get_pagetable_gmap.
-    rewrite lookup_delete_ne;eauto.
-    apply elem_of_list_to_map_1.
-    {  rewrite -list_fmap_compose /compose /=. rewrite list_fmap_id. apply NoDup_list_of_vmids. }
-    rewrite elem_of_list_In.
-    rewrite in_map_iff.
-    exists j.
-    split.
-    rewrite /get_pagetable_gset //.
-    apply in_list_of_vmids.
+  Lemma access_split_set_diff {p} q1 q2 (s1 s2 : gset VMID):
+   s2 ⊆ s1 -> A@p:={(q1+q2)%Qp} [s1] -∗ A@p:={q1} [s2] ∗ A@p:={q2} [s1 ∖ s2].
+  Proof using.
+    iIntros (Hsub) "HO".
+    rewrite access_mapsto_eq.
+    iApply own_op.
+    rewrite -auth_frag_op singleton_op.
+    rewrite -pair_op.
+    rewrite (gset_disj_union _ _);
+    last set_solver+ .
+    rewrite -(union_difference_L _ _ Hsub).
+    naive_solver.
   Qed.
 
-  Lemma gen_pagetable_valid_pure{Perm: Type} {σ i q γ} proj (checkb: Perm -> bool) (s:gset PID):
-   ghost_map_auth γ 1 (get_pagetable_gmap σ proj checkb)  -∗
-   ghost_map_elem γ i (DfracOwn q) s -∗
-   ⌜(get_pagetable_gmap σ proj checkb) !! i = Some s ⌝.
+
+ (* Lemma gen_pagetable_SepM_split1 {Perm: Type} {σ γ} i (proj: page_table -> gmap PID Perm) *)
+ (*        (checkb: Perm -> bool): *)
+ (*   ([∗ map] k↦v ∈ (get_pagetable_gmap σ proj checkb ), ghost_map_elem γ k (dfrac.DfracOwn 1) v)%I -∗ *)
+ (*   ghost_map_elem γ i (dfrac.DfracOwn 1) (get_pagetable_gset σ i proj checkb) ∗ *)
+ (*   [∗ map] k↦v ∈ (delete i (get_pagetable_gmap σ proj checkb)), ghost_map_elem γ k (dfrac.DfracOwn 1) v. *)
+ (*  Proof. *)
+ (*    iIntros "Hall". *)
+ (*    iApply ((big_sepM_delete _ (get_pagetable_gmap σ proj checkb) i *)
+ (*                             (get_pagetable_gset σ i proj checkb)) with "Hall"). *)
+ (*    rewrite /get_pagetable_gmap. *)
+ (*    apply elem_of_list_to_map_1. *)
+ (*    {  rewrite -list_fmap_compose /compose /=. rewrite list_fmap_id. apply NoDup_list_of_vmids. } *)
+ (*    rewrite elem_of_list_In. *)
+ (*    rewrite in_map_iff. *)
+ (*    exists i. *)
+ (*    split. *)
+ (*    rewrite /get_pagetable_gset //. *)
+ (*    apply in_list_of_vmids. *)
+ (*  Qed. *)
+
+ (*  Lemma gen_pagetable_SepM_split2 {Perm: Type} {σ γ} i j (proj: page_table -> gmap PID Perm) *)
+ (*        (checkb: Perm -> bool): *)
+ (*   i ≠ j -> *)
+ (*   ([∗ map] k↦v ∈ (get_pagetable_gmap σ proj checkb ), ghost_map_elem γ k (dfrac.DfracOwn 1) v)%I -∗ *)
+ (*   ghost_map_elem γ i (dfrac.DfracOwn 1) (get_pagetable_gset σ i proj checkb) ∗ *)
+ (*   ghost_map_elem γ j (dfrac.DfracOwn 1) (get_pagetable_gset σ j proj checkb) ∗ *)
+ (*   [∗ map] k↦v ∈ (delete j (delete i (get_pagetable_gmap σ proj checkb))), *)
+ (*                  ghost_map_elem γ k (dfrac.DfracOwn 1) v. *)
+ (*  Proof. *)
+ (*    iIntros (Hne) "Hall". *)
+ (*    iDestruct ((gen_pagetable_SepM_split1 i) with "Hall") as "[Hi Hrest]". *)
+ (*    iFrame. *)
+ (*    iApply ((big_sepM_delete _ _ j (get_pagetable_gset σ j proj checkb)) with "Hrest"). *)
+ (*    rewrite /get_pagetable_gmap. *)
+ (*    rewrite lookup_delete_ne;eauto. *)
+ (*    apply elem_of_list_to_map_1. *)
+ (*    {  rewrite -list_fmap_compose /compose /=. rewrite list_fmap_id. apply NoDup_list_of_vmids. } *)
+ (*    rewrite elem_of_list_In. *)
+ (*    rewrite in_map_iff. *)
+ (*    exists j. *)
+ (*    split. *)
+ (*    rewrite /get_pagetable_gset //. *)
+ (*    apply in_list_of_vmids. *)
+ (*  Qed. *)
+
+  Lemma gen_owned_valid_pure {σ q γ} p s:
+   ghost_map_auth γ 1 (get_owned_gmap σ)  -∗
+   ghost_map_elem γ p (DfracOwn q) s -∗
+   ⌜(get_owned_gmap σ) !! p = Some s ⌝.
   Proof.
     iIntros  "Hσ Hpt".
+    iApply (ghost_map_lookup with "Hσ Hpt").
+  Qed.
+
+  Lemma gen_access_valid_pure {σ γ} p q s:
+   own γ (● (get_access_gmap σ)) -∗
+   own γ (◯ {[p := (q, (GSet s))]}) -∗
+   ⌜(get_access_gmap σ) !! p = Some (q, (GSet s)) ⌝.
+  Proof.
+    iIntros  "Hσ Hpt".
+    iDestruct (own_valid_2 with "Hσ Hpt") as "%Hvalid".
+
+    apply auth_frag_valid in Hvalid.
+
     iApply (ghost_map_lookup with "Hσ Hpt").
   Qed.
 
