theories/lang/pagetable_extra.v
@@ -5,352 +5,191 @@ Section pagetable_extra.
 
 Context `{HyperConst : HypervisorConstants}.
 
-Lemma update_ownership_batch_preserve_current_vm σ (ps: list PID) perm:
- get_current_vm (update_ownership_batch σ ps perm) = get_current_vm σ.
+Lemma update_ownership_batch_preserve_current_vm σ (ps: list PID):
+ get_current_vm (update_ownership_batch σ ps) = get_current_vm σ.
 Proof. f_equal. Qed.
 
-Lemma update_ownership_batch_preserve_regs σ (ps: list PID) perm:
- get_reg_gmap (update_ownership_batch σ ps perm) = get_reg_gmap σ.
+Lemma update_ownership_batch_preserve_regs σ (ps: list PID):
+ get_reg_gmap (update_ownership_batch σ ps) = get_reg_gmap σ.
 Proof. f_equal. Qed.
 
-Lemma update_ownership_batch_preserve_mem σ (ps: list PID) perm:
- get_mem (update_ownership_batch σ ps perm) = get_mem σ.
+Lemma update_ownership_batch_preserve_mem σ (ps: list PID):
+ get_mem (update_ownership_batch σ ps) = get_mem σ.
 Proof. f_equal. Qed.
 
-Lemma update_ownership_batch_preserve_tx σ (ps: list PID) perm:
- get_tx_agree (update_ownership_batch σ ps perm) = get_tx_agree σ.
+Lemma update_ownership_batch_preserve_rx σ (ps: list PID):
+ get_rx_gmap (update_ownership_batch σ ps) = get_rx_gmap σ.
 Proof. f_equal. Qed.
 
-Lemma update_ownership_batch_preserve_rx1 σ (ps: list PID) perm:
- get_rx_agree (update_ownership_batch σ ps perm) = get_rx_agree σ.
+Lemma update_ownership_batch_preserve_trans σ (ps: list PID):
+ get_trans_gmap (update_ownership_batch σ ps) = get_trans_gmap σ.
+Proof.  f_equal. Qed.
+
+Lemma update_ownership_batch_preserve_trans' σ (ps: list PID):
+ get_transactions (update_ownership_batch σ ps) = get_transactions σ.
 Proof. f_equal. Qed.
 
-Lemma update_ownership_batch_preserve_rx2 σ (ps: list PID) perm:
- get_rx_gmap (update_ownership_batch σ ps perm) = get_rx_gmap σ.
+Lemma update_ownership_batch_preserve_hpool σ (ps: list PID):
+ get_hpool_gset (update_ownership_batch σ ps) = get_hpool_gset σ.
 Proof. f_equal. Qed.
 
-Lemma update_ownership_batch_preserve_rx σ (ps: list PID) perm:
- (get_rx_agree (update_ownership_batch σ ps perm), get_rx_gmap (update_ownership_batch σ ps perm) ) =
- (get_rx_agree σ, get_rx_gmap σ).
-Proof. by rewrite update_ownership_batch_preserve_rx1 update_ownership_batch_preserve_rx2 . Qed.
-
-Lemma update_ownership_batch_preserve_trans σ (ps: list PID) perm:
- get_trans_gmap (update_ownership_batch σ ps perm) = get_trans_gmap σ.
+Lemma update_ownership_batch_preserve_retri σ (ps: list PID):
+ get_retri_gmap (update_ownership_batch σ ps) = get_retri_gmap σ.
 Proof. f_equal. Qed.
 
-Lemma update_ownership_batch_preserve_trans' σ (ps: list PID) perm:
- get_transactions (update_ownership_batch σ ps perm) = get_transactions σ.
-Proof. f_equal. Qed.
-
-Lemma update_ownership_batch_preserve_hpool σ (ps: list PID) perm:
- get_hpool_gset (update_ownership_batch σ ps perm) = get_hpool_gset σ.
-Proof. f_equal. Qed.
-
-Lemma update_ownership_batch_preserve_retri σ (ps: list PID) perm:
- get_retri_gmap (update_ownership_batch σ ps perm) = get_retri_gmap σ.
-Proof. f_equal. Qed.
-
-Lemma update_ownership_batch_preserve_other_page_tables σ ps perm i:
- i ≠ (get_current_vm σ) ->
- (get_page_tables (update_ownership_batch σ ps perm)) !!! i =
- (get_page_tables σ) !!! i.
+Lemma update_ownership_batch_preserve_access σ ps:
+((get_access_gmap (update_ownership_batch σ ps)):gmap _ _) = ((get_access_gmap σ): gmap _ _).
 Proof.
-  intros.
-  rewrite /get_page_tables /update_ownership_batch /update_ownership_global_batch /=.
-  rewrite vlookup_insert_ne.
-  rewrite /get_page_tables //.
+  rewrite /get_access_gmap /update_ownership_batch /update_ownership_global_batch /get_page_table /=.
+  generalize dependent σ.
+  induction ps.
   done.
+  simpl.
+  intro.
+  rewrite /update_ownership' /=.
+  destruct (list.foldr
+      (λ (p : PID) (acc : page_table),
+         match acc !! p with
+         | Some (_, s) => <[p:= (get_current_vm σ, s)]> acc
+         | None => acc
+         end) σ.1.1.1.2 ps !! a) eqn:Hlookup.
+  { destruct p.
+    rewrite fmap_insert.
+    rewrite IHps /=.
+    assert (∃ v', σ.1.1.1.2 !! a = Some (v', g)).
+    { clear IHps.
+      generalize dependent v.
+      induction ps;intros v Hlookup; simpl in Hlookup.
+      exists v;done.
+      destruct (list.foldr
+                (λ (p : PID) (acc : page_table),
+                   match acc !! p with
+                   | Some (_, s) => <[p:= (get_current_vm σ, s)]> acc
+                   | None => acc
+                   end) σ.1.1.1.2 ps !! a0) eqn: Hlookup'.
+      { destruct p.
+        destruct (decide (a0=a)).
+        subst a0.
+        apply (IHps v0).
+        rewrite lookup_insert in Hlookup.
+        inversion Hlookup.
+        subst g0.
+        done.
+        rewrite lookup_insert_ne in Hlookup;[|done].
+        apply (IHps v Hlookup).
+      }
+      { apply (IHps v Hlookup).
+      }
+    }
+    destruct H.
+    apply map_eq.
+    intro.
+    destruct (decide (i=a)).
+    rewrite e.
+    rewrite lookup_insert.
+    rewrite lookup_fmap H.
+    done.
+    rewrite lookup_insert_ne;[done|eauto].
+  }
+  rewrite IHps //.
 Qed.
 
-Lemma update_ownership_batch_preserve_access σ ps perm : get_access_gmap (update_ownership_batch σ ps perm) = (get_access_gmap σ).
+Lemma update_access_batch_preserve_current_vm σ (ps: list PID) :
+ get_current_vm (update_access_batch σ ps) = get_current_vm σ.
+Proof. f_equal. Qed.
+
+Lemma update_access_batch_preserve_regs σ (ps: list PID):
+ get_reg_gmap (update_access_batch σ ps) = get_reg_gmap σ.
+Proof. f_equal. Qed.
+
+Lemma update_access_batch_preserve_mem σ (ps: list PID):
+ get_mem (update_access_batch σ ps) = get_mem σ.
+Proof. f_equal. Qed.
+
+Lemma update_access_batch_preserve_rx σ (ps: list PID):
+ get_rx_gmap (update_access_batch σ ps) = get_rx_gmap σ.
+Proof. f_equal. Qed.
+
+Lemma update_access_batch_preserve_trans σ (ps: list PID) :
+ get_trans_gmap (update_access_batch σ ps) = get_trans_gmap σ.
+Proof. f_equal. Qed.
+
+Lemma update_access_batch_preserve_trans' σ (ps: list PID):
+ get_transactions (update_access_batch σ ps) = get_transactions σ.
+Proof. f_equal. Qed.
+
+Lemma update_access_batch_preserve_hpool σ (ps: list PID):
+ get_hpool_gset (update_access_batch σ ps) = get_hpool_gset σ.
+Proof. f_equal. Qed.
+
+Lemma update_access_batch_preserve_retri σ (ps: list PID):
+ get_retri_gmap (update_access_batch σ ps) = get_retri_gmap σ.
+Proof. f_equal. Qed.
+
+Lemma update_access_batch_preserve_ownerships σ ps:
+ (get_owned_gmap (update_access_batch σ ps)) = (get_owned_gmap σ).
 Proof.
-  rewrite /get_access_gmap /get_pagetable_gmap /update_ownership_batch /update_ownership_global_batch /=.
-  f_equal.
-  simplify_list_eq.
-  apply (list_eq_same_length _ _ vm_count).
-  rewrite fmap_length.
-  apply length_list_of_vmids.
-  rewrite fmap_length.
-  apply length_list_of_vmids.
-  intros.
-  apply list_lookup_fmap_inv in H0, H1.
-  destruct H0, H1.
-  destruct H0, H1.
-  rewrite H3 in H2.
-  inversion H2;subst x1.
-  clear H2.
-  rewrite H0 H1 /get_pagetable_gset.
-  do 5 f_equal.
-  rewrite /get_vm_page_table /get_page_tables /=.
-  destruct (decide (get_current_vm σ = x0)).
-  subst x0.
-  rewrite vlookup_insert //.
-  rewrite vlookup_insert_ne //.
-Qed.
-
-Lemma update_ownership_batch_preserve_excl σ ps perm : get_excl_gmap (update_ownership_batch σ ps perm) = (get_excl_gmap σ).
-Proof.
-  rewrite /get_excl_gmap /get_pagetable_gmap /update_ownership_batch /update_ownership_global_batch /=.
-  f_equal.
-  simplify_list_eq.
-  apply (list_eq_same_length _ _ vm_count).
-  rewrite fmap_length.
-  apply length_list_of_vmids.
-  rewrite fmap_length.
-  apply length_list_of_vmids.
-  intros.
-  apply list_lookup_fmap_inv in H0, H1.
-  destruct H0, H1.
-  destruct H0, H1.
-  rewrite H3 in H2.
-  inversion H2;subst x1.
-  clear H2.
-  rewrite H0 H1 /get_pagetable_gset.
-  do 5 f_equal.
-  rewrite /get_vm_page_table /get_page_tables /=.
-  destruct (decide (get_current_vm σ = x0)).
-  subst x0.
-  rewrite vlookup_insert //.
-  rewrite vlookup_insert_ne //.
-Qed.
-
-
-
-Lemma update_access_batch_preserve_current_vm σ (ps: list PID) perm:
- get_current_vm (update_access_batch σ ps perm) = get_current_vm σ.
-Proof. f_equal. Qed.
-
-Lemma update_access_batch_preserve_regs σ (ps: list PID) perm:
- get_reg_gmap (update_access_batch σ ps perm) = get_reg_gmap σ.
-Proof. f_equal. Qed.
-
-Lemma update_access_batch_preserve_mem σ (ps: list PID) perm:
- get_mem (update_access_batch σ ps perm) = get_mem σ.
-Proof. f_equal. Qed.
-
-Lemma update_access_batch_preserve_tx σ (ps: list PID) perm:
- get_tx_agree (update_access_batch σ ps perm) = get_tx_agree σ.
-Proof. f_equal. Qed.
-
-Lemma update_access_batch_preserve_rx1 σ (ps: list PID) perm:
- get_rx_agree (update_access_batch σ ps perm) = get_rx_agree σ.
-Proof. f_equal. Qed.
-
-Lemma update_access_batch_preserve_rx2 σ (ps: list PID) perm:
- get_rx_gmap (update_access_batch σ ps perm) = get_rx_gmap σ.
-Proof. f_equal. Qed.
-
-Lemma update_access_batch_preserve_rx σ (ps: list PID) perm:
- (get_rx_agree (update_access_batch σ ps perm), get_rx_gmap (update_access_batch σ ps perm) ) =
- (get_rx_agree σ, get_rx_gmap σ).
-Proof. by rewrite update_access_batch_preserve_rx1 update_access_batch_preserve_rx2. Qed.
-
-Lemma update_access_batch_preserve_trans σ (ps: list PID) perm:
- get_trans_gmap (update_access_batch σ ps perm) = get_trans_gmap σ.
-Proof. f_equal. Qed.
-
-Lemma update_access_batch_preserve_trans' σ (ps: list PID) perm:
- get_transactions (update_access_batch σ ps perm) = get_transactions σ.
-Proof. f_equal. Qed.
-
-Lemma update_access_batch_preserve_hpool σ (ps: list PID) perm:
- get_hpool_gset (update_access_batch σ ps perm) = get_hpool_gset σ.
-Proof. f_equal. Qed.
-
-Lemma update_access_batch_preserve_retri σ (ps: list PID) perm:
- get_retri_gmap (update_access_batch σ ps perm) = get_retri_gmap σ.
-Proof. f_equal. Qed.
-
-Lemma update_access_batch_preserve_other_page_tables σ ps perm i:
- i ≠ (get_current_vm σ) ->
- (get_page_tables (update_access_batch σ ps perm)) !!! i =
- (get_page_tables σ) !!! i.
-Proof.
-  intros.
-  rewrite /get_page_tables /update_access_batch /update_access_global_batch /=.
-  rewrite vlookup_insert_ne.
-  rewrite /get_page_tables //.
+  rewrite /get_owned_gmap /update_access_batch /update_access_global_batch /get_page_table /=.
+  do 2 f_equal.
+  generalize dependent σ.
+  induction ps.
   done.
+  simpl.
+  intro.
+  rewrite /update_access' /=.
+  destruct (list.foldr
+      (λ (p : PID) (acc : page_table),
+         match acc !! p with
+         | Some (o, s) => <[p:= (o, {[get_current_vm σ]} ∪ s)]> acc
+         | None => acc
+         end) σ.1.1.1.2 ps !! a) eqn:Hlookup.
+  { destruct p.
+    rewrite fmap_insert.
+    rewrite IHps /=.
+    assert (∃ g', σ.1.1.1.2 !! a = Some (v, g')).
+    { clear IHps.
+      generalize dependent g.
+      induction ps;intros g Hlookup; simpl in Hlookup.
+      exists g;done.
+      destruct (list.foldr
+                (λ (p : PID) (acc : page_table),
+                   match acc !! p with
+                   | Some (o, s) => <[p:= (o, {[get_current_vm σ]} ∪ s)]> acc
+                   | None => acc
+                   end) σ.1.1.1.2 ps !! a0) eqn: Hlookup'.
+      { destruct p.
+        destruct (decide (a0=a)).
+        subst a0.
+        apply (IHps g0).
+        rewrite lookup_insert in Hlookup.
+        inversion Hlookup.
+        subst v0.
+        done.
+        rewrite lookup_insert_ne in Hlookup;[|done].
+        apply (IHps g Hlookup).
+      }
+      { apply (IHps g Hlookup).
+      }
+    }
+    destruct H.
+    apply map_eq.
+    intro.
+    destruct (decide (i=a)).
+    rewrite e.
+    rewrite lookup_insert.
+    rewrite lookup_fmap H.
+    done.
+    rewrite lookup_insert_ne;[done|eauto].
+  }
+  rewrite IHps //.
 Qed.
 
-Lemma update_access_batch_preserve_ownerships σ ps perm :
- (get_owned_gmap (update_access_batch σ ps perm)) = (get_owned_gmap σ).
-Proof.
-  rewrite /get_owned_gmap /get_pagetable_gmap /update_access_batch /update_access_global_batch /=.
-  f_equal.
-  simplify_list_eq.
-  apply (list_eq_same_length _ _ vm_count).
-  rewrite fmap_length.
-  apply length_list_of_vmids.
-  rewrite fmap_length.
-  apply length_list_of_vmids.
-  intros.
-  apply list_lookup_fmap_inv in H0, H1.
-  destruct H0, H1.
-  destruct H0, H1.
-  rewrite H3 in H2.
-  inversion H2;subst x1.
-  clear H2.
-  rewrite H0 H1 /get_pagetable_gset.
-  do 5 f_equal.
-  rewrite /get_vm_page_table /get_page_tables /=.
-  destruct (decide (get_current_vm σ = x0)).
-  subst x0.
-  rewrite vlookup_insert //.
-  rewrite vlookup_insert_ne //.
-Qed.
+(* TODO: update_access_batch_preserve_mb (easy) *)
+(* TODO: update_ownership_batch_preserve_mb (hard) *)
+(* TODO: *)
 
-(* TODO rename hypotheses. *)
-Lemma update_access_batch_preserve_excl {sps sexcl:gset _} σ ps:
- sps = (list_to_set ps)->
- get_excl_gmap σ !! (get_current_vm σ) = Some sexcl ->
- sps ## sexcl ->
- (get_excl_gmap (update_access_batch σ ps SharedAccess)) = (get_excl_gmap σ).
-Proof.
-  rewrite /get_excl_gmap /get_pagetable_gmap.
-  intros.
-  f_equal.
-  apply (list_eq_same_length _ _ vm_count).
-  - rewrite map_length.
-    apply length_list_of_vmids.
-  - rewrite map_length.
-    apply length_list_of_vmids.
-  - intros ? ? ? Hlt Hl1 Hl2.
-    rewrite list_lookup_fmap /=in Hl1.
-    pose proof (lookup_list_of_vmids i Hlt) as Hv.
-    rewrite Hv /=in Hl1.
-    inversion Hl1.
-    rewrite list_lookup_fmap /=in Hl2.
-    rewrite Hv /= in Hl2.
-    inversion Hl2.
-    f_equal.
-    apply elem_of_list_to_map_2 in H0.
-    apply elem_of_list_In in H0.
-    apply in_map_iff in H0.
-    destruct H0 as [?[Heq _]].
-    inversion Heq.
-    subst x0.
-    set (v:= (nat_to_fin Hlt)) in *.
-    clear Hl1 Hl2 H3 H4 Heq.
-    destruct (decide ((get_current_vm σ) = v)).
-    + rewrite e in H5. rewrite H5.
-      rewrite /get_pagetable_gset /=.
-      apply set_eq.
-      intros.
-      split.
-      *  rewrite elem_of_list_to_set.
-         intro.
-         apply elem_of_list_In in H0.
-         apply in_map_iff in H0.
-         destruct H0 as [? [<- Hin]].
-         apply elem_of_list_In in Hin.
-         destruct x1.
-         apply elem_of_map_to_list in Hin.
-         apply map_filter_lookup_Some in Hin.
-         destruct Hin.
-         rewrite -H5 /get_pagetable_gset /=.
-         rewrite elem_of_list_to_set.
-         apply elem_of_list_In.
-         apply in_map_iff.
-         exists (p,a).
-         split;auto.
-         apply elem_of_list_In.
-         apply elem_of_map_to_list.
-         apply map_filter_lookup_Some.
-         split;auto.
-         rewrite /get_vm_page_table /get_page_tables /= in H0.
-         rewrite -e in H0.
-         rewrite vlookup_insert /=in H0.
-         generalize dependent  sps.
-         induction ps.
-         cbn in H0.
-         rewrite -e //.
-         intros.
-         cbn in H0.
-         destruct (decide (a0 = p)).
-         subst a0.
-         rewrite lookup_insert in H0.
-         inversion H0.
-         subst a.
-         cbn in H2.
-         done.
-         rewrite lookup_insert_ne in H0.
-         apply (IHps H0 (list_to_set ps));auto.
-         cbn in H.
-         subst sps.
-         apply disjoint_union_l  in H1.
-         destruct H1.
-         assumption.
-         done.
-      *  rewrite elem_of_list_to_set.
-         intro.
-         rewrite -H5 in H0.
-         rewrite /get_pagetable_gset /get_vm_page_table /get_page_tables /= in H0.
-         apply elem_of_list_to_set in H0.
-         apply elem_of_list_In in H0.
-         apply in_map_iff in H0.
-         destruct H0 as [? [<- Hin]].
-         apply elem_of_list_In in Hin.
-         destruct x1.
-         apply elem_of_map_to_list in Hin.
-         apply map_filter_lookup_Some in Hin.
-         destruct Hin.
-         apply elem_of_list_In.
-         apply in_map_iff.
-         exists (p,a).
-         split;auto.
-         apply elem_of_list_In.
-         apply elem_of_map_to_list.
-         apply map_filter_lookup_Some.
-         split;auto.
-         rewrite /get_vm_page_table /get_page_tables /=.
-         rewrite -e.
-         rewrite vlookup_insert /=.
-         generalize dependent  sps.
-         induction ps.
-         intros.
-         cbn.
-         rewrite e //.
-         intros.
-         cbn.
-         destruct (decide (a0 = p)).
-         -- assert (Hpin: p ∈ sexcl ).
-            {
-              rewrite -H5.
-              rewrite /get_pagetable_gset /get_vm_page_table /get_page_tables /=.
-              apply elem_of_list_to_set.
-              apply elem_of_list_In.
-              apply in_map_iff.
-              exists (p,a).
-              split;auto.
-              apply elem_of_list_In.
-              apply elem_of_map_to_list.
-              apply map_filter_lookup_Some.
-              split;done.
-            }
-            subst a0.
-            assert (Hpin': p ∈ sps).
-            {
-              set_solver.
-            }
-            set_solver.
-         --
-         rewrite lookup_insert_ne;auto.
-         apply (IHps (list_to_set ps));auto.
-         cbn in H.
-         subst sps.
-         apply disjoint_union_l  in H1.
-         destruct H1.
-         assumption.
-    + rewrite /get_pagetable_gset /=.
-      do 3 f_equal.
-      rewrite /get_vm_page_table /get_page_tables /update_access_batch /update_access_global_batch /=.
-      rewrite vlookup_insert_ne;auto.
-    Qed.
-
-
-Lemma get_pagetable_gmap_checkb {Perm:Type} {σ i s} proj (checkb: Perm -> bool) p:
- (get_pagetable_gmap σ proj checkb) !! i = Some  s->
+Lemma get_pagetable_gmap_checkb {σ} p v s:
+ (get_pagetable_gmap σ) !! p = Some (v, s)->
  (p ∈ s <->
   ∃ perm, (proj (get_vm_page_table σ i)) !! p =Some perm ∧ checkb perm = true).
 Proof.
